gref is added to state and api signatures simplified

share/pulse/examples/dice/dpe/SPDM3.fst
@@ -43,31 +43,30 @@ module PHT = Pulse.Lib.HashTable.Spec
 open PulseCore.Preorder
 open Pulse.Lib.OnRange
 
-let trace_ref = admit ()
 
 let pcm_elt (p:perm) (t:trace) : pcm_t = Some p, t
 
 fn init0 (key_size:u32) (signing_pub_key:V.vec u8 { V.length signing_pub_key == U32.v key_size })
   (#s:Seq.seq u8)
   requires V.pts_to signing_pub_key s
-  returns r:state & gref
-  ensures init_inv key_size s (fst r) (snd r)
+  returns r:state 
+  ensures init_inv key_size s r
 {
   //creation of session_transcript
   let session_transcript = V.alloc 0uy 0sz;
   
-  //creation of the session data storage
-  let st = { key_size; signing_pub_key; session_transcript };
-  
   //creation of the ghost session data storage
   let repr = {key_size_repr = key_size; signing_pub_key_repr = s; transcript = Seq.empty};
-  
+
   //creation of the trace
   let trace = next_trace emp_trace (G_Initialized repr);
-  
+
   //creation of the ghost trace ref
   let r = ghost_alloc #_ #trace_pcm (pcm_elt 1.0R trace);
- 
+
+  //creation of the session data storage
+  let st = { key_size; signing_pub_key; session_transcript;g_trace_ref = r };
+  
   (*Current context:
     ghost_pcm_pts_to r (G.reveal (G.hide (pcm_elt 1.0R trace))) **
     V.pts_to session_transcript (Seq.Base.create (SZ.v 0sz) 0uy) **
@@ -109,12 +108,12 @@ fn init0 (key_size:u32) (signing_pub_key:V.vec u8 { V.length signing_pub_key == 
    (*Current context:
     spdm_inv (Initialized st) r trace*)
 
-  let res = (Initialized st, r);
+  let res = Initialized st;
 
   (*Current context:
     pure (res == (Initialized st, r)) ** spdm_inv (Initialized st) r trace*)
 
-  fold (init_inv key_size s (fst res) (snd res));
+  fold (init_inv key_size s (Initialized st));
 
   (*Current context:
     init_inv key_size s (fst res) (snd res)*)
@@ -122,73 +121,37 @@ fn init0 (key_size:u32) (signing_pub_key:V.vec u8 { V.length signing_pub_key == 
   res
 }
 
-let b_resp_resp_repr_relation (req_param1: u8)
-                              (req_param2:u8) (measurementspecification: u8) 
-                              (req_context: Seq.seq u8{Seq.length req_context == 8})
-                              (r:resp_repr req_param1 req_param2 measurementspecification req_context) (s:Seq.seq u8) =
+let b_resp_resp_repr_relation (ctx:parser_context)
+                              (r:resp_repr ctx) 
+                              (s:Seq.seq u8) =
 
 admit()
 
-let valid_resp_bytes (req_param1: u8)
-                            (req_param2:u8) (measurementspecification: u8) 
-                            (req_context: Seq.seq u8{Seq.length req_context == 8})
-                            (b:Seq.seq u8) 
-                            (r:resp_repr req_param1 req_param2 measurementspecification req_context) =
+let valid_resp_bytes (ctx:parser_context)
+                     (b:Seq.seq u8) 
+                     (r:resp_repr ctx) =
 admit()
 
-type parser_context = {
-  req_param1 : u8;
-  req_param2 : u8;
-  req_context0 : u8;
-  req_context1 : u8;
-  req_context2 : u8;
-  m_spec : u8
-}
-
-assume val resp_repr0 (ctx:parser_context) : Type0
-assume val valid_resp_bytes0 (ctx:parser_context) (s:Seq.seq u8) (r:resp_repr0 ctx) : slprop
-assume val blocks_of_resp_repr (#ctx:parser_context) (r:resp_repr0 ctx)
-  : GTot (Seq.seq (measurement_block_repr ctx.req_param2 ctx.m_spec))
-assume val valid_measurement_blocks0
+fn parser0 
   (ctx:parser_context)
-  (s:Seq.seq (measurement_block_repr ctx.req_param2 ctx.m_spec)) : slprop
-
-let parser_post (ctx:parser_context) (s:Seq.seq u8) (res:spdm_measurement_result_t) =
-  match res.status with
-  | Parse_error -> pure True
-  | Signature_verification_error -> pure False
-  | Success ->
-    exists* (r:resp_repr0 ctx).
-    valid_resp_bytes0 ctx s r **
-    valid_measurement_blocks0 ctx (blocks_of_resp_repr r)
-
-fn parser0
-  (ctx:parser_context)
-  (resp_size: u32)
-  (resp:V.vec u8 { V.length resp == u32_v resp_size })
   (#p:perm)
-  (#s:Ghost.erased (Seq.seq u8))
-    
-  requires V.pts_to resp #p s
-  returns res:spdm_measurement_result_t
-  ensures 
-    V.pts_to resp #p s **
-    parser_post ctx s res
+  (#b_resp: G.erased (Seq.seq u8))
+
+requires V.pts_to ctx.resp #p b_resp
+returns res: spdm_measurement_result_t 
+ensures 
+         V.pts_to ctx.resp #p b_resp **
+         parser_post ctx res #b_resp
 {
-  admit ()
+  admit()
 }
 
+let get_state_data_transcript (s_data:st) : V.vec u8 = s_data.session_transcript
 
-let get_state_data (c:state) =
-  match c with
-  | Initialized s -> s
-  | Recv_no_sign_resp s -> s
+let get_state_data_signing_pub_key (s_data:st) : V.vec u8 = s_data.signing_pub_key
 
-let get_state_data_transcript (s_data:st) = s_data.session_transcript
+let get_state_data_key_size (s_data:st) : u32 = s_data.key_size
 
-let get_state_data_signing_pub_key (s_data:st) = s_data.signing_pub_key
-
-let get_state_data_key_size (s_data:st) = s_data.key_size
 
 //We have taken permissions on v1 and v2 and if we are not returning v1 nad v2, then the client losts this permission and then
 //the client will not be able to deallocate v1 and v2. Read permissions.
@@ -196,13 +159,14 @@ fn append_vec
   (#a:Type0)
   (v1: V.vec a)
   (v2: V.vec a)
-  (#p1:perm)
-  (#p2:perm)
   (#v1_seq: Ghost.erased (Seq.seq a)) //put G.erased
   (#v2_seq: Ghost.erased (Seq.seq a))
+  (#p1:perm)
+  (#p2:perm)
   
   requires V.pts_to v1 #p1 v1_seq **
            V.pts_to v2 #p2 v2_seq
+
   returns v:V.vec a
   ensures V.pts_to v (Seq.append v1_seq v2_seq) **
           V.pts_to v1 #p1 v1_seq **
@@ -211,144 +175,44 @@ fn append_vec
     admit()
   }      
 
-#push-options "--query_stats"
+fn parser 
+(ctx:parser_context)
+(#p:perm)
+(#b_resp: G.erased (Seq.seq u8))  
+requires V.pts_to ctx.resp #p b_resp
+ returns res: spdm_measurement_result_t 
+ensures V.pts_to ctx.resp #p b_resp **
+                        parser_post ctx res #b_resp
 
-// (pure ((G_Recv_no_sign_resp? (current_state tr1) /\
-//                                                  valid_transition tr0 (current_state tr1) /\ tr1 == next_trace tr0 (current_state tr1)) /\
-//                                                  (G_Recv_no_sign_resp? (current_state tr1) /\
-                                               
-//                                                   g_transcript_current_session_grows_by (current_transcript tr0 ) 
-//                                                                                      (current_transcript tr1) 
-//                                                                                      (Seq.append b_req b_resp))))
-assume val valid_trace_for_no_sign_resp (tr0 tr1:trace) : prop
+{
+  admit()
+}
+
+let no_sign_resp_state_related_post_conditions 
+  (ctx:parser_context)
+  (r:resp_repr ctx)
+  (tr0:trace)
+  (tr1:trace)
+  (c:state)
+  (res_state:state) 
+  (#b_resp: Seq.seq u8)
+  (#b_req: Seq.seq u8) =
+valid_resp0 ctx r **
+spdm_inv c (get_state_data res_state).g_trace_ref tr1 **
+
+(pure ((G_Recv_no_sign_resp? (current_state tr1) /\
+valid_transition tr0 (current_state tr1) /\ tr1 == next_trace tr0 (current_state tr1)) /\
+(G_Recv_no_sign_resp? (current_state tr1) /\
+g_transcript_current_session_grows_by (current_transcript tr0 ) 
+                                      (current_transcript tr1) 
+                                      (Seq.append b_req b_resp))))
+
+
 
 fn no_sign_resp1
   (ctx:parser_context)
   (req_size: u32)
-  (resp_size: u32)
   (req:V.vec u8 { V.length req == u32_v req_size })
-  (resp:V.vec u8 { V.length resp == u32_v resp_size })
-  (c:state)
-  (#tr0:trace{has_full_state_info (current_state tr0)})
-  (#p_req:perm)
-  (#p_resp:perm)
-  (#b_resp:G.erased (Seq.seq u8))
-  (#b_req:G.erased (Seq.seq u8))
-  
-  requires V.pts_to req #p_req b_req **
-           V.pts_to resp #p_resp b_resp **
-           spdm_inv c trace_ref tr0 **
-           pure (G_Recv_no_sign_resp? (current_state tr0) \/ G_Initialized? (current_state tr0))
-  
-  returns res:spdm_measurement_result_t & state
-    
-  ensures V.pts_to req #p_req b_req **
-          V.pts_to resp #p_resp b_resp **
-          (match (fst res).status with
-           | Parse_error -> pure True
-           | Signature_verification_error -> pure False
-           | Success ->
-             //parser post-condition 
-             (exists* r. valid_resp_bytes0 ctx b_resp r **
-                         valid_measurement_blocks0 ctx (blocks_of_resp_repr r)) **
-                              
-             //state change related post-condition 
-             (exists* tr1. spdm_inv c trace_ref tr1 **
-                           pure (valid_trace_for_no_sign_resp tr0 tr1)))
-                                         
-
-{
-  let res = parser0 ctx resp_size resp;
-
-  match res.status {
-    Parse_error -> {
-      admit ()
-    }
-    Signature_verification_error -> {
-      rewrite (parser_post ctx b_resp res) as
-              (pure False);
-      unreachable ()
-    }
-    Success -> {
-      admit ()
-    }
-  }
-
-  // //current state transcript
-  // let curr_state_data = get_state_data c;
-  // let curr_state_transcript = get_state_data_transcript curr_state_data;
-  // let curr_state_signing_pub_key = get_state_data_signing_pub_key curr_state_data;
-  // let curr_state_key_size = get_state_data_key_size curr_state_data;
-
-  
-  // //append req and resp
-  // let append_req_resp = append_vec req resp #b_req #b_resp #p_req #p_resp;
-  
-  // //get the ghost transcript
-  // let curr_g_transcript = current_transcript tr0;
-  // let curr_g_key = current_key tr0;
-  // let curr_g_key_size = current_key_size tr0;
-  // //unfold (spdm_inv c trace_ref tr0);
-  
-  // //unfold (session_state_related c (current_state tr0));
-
-  // assume_(V.pts_to curr_state_transcript (G.reveal curr_g_transcript));
-  // //append req/resp to the current trascript
-  // let new_transcript = append_vec curr_state_transcript append_req_resp #curr_g_transcript #(Seq.append b_req b_resp);
-  // let new_g_transcript = g_append curr_g_transcript (Seq.append b_req b_resp);
-  // //create a new state data record with the new transcript
-  // assume_ (pure (V.length curr_state_signing_pub_key == u32_v curr_state_key_size));
-
-  // let new_st = {key_size = curr_state_key_size; signing_pub_key = curr_state_signing_pub_key; session_transcript = new_transcript };
-  
-  // ////creation of the ghost session data storage
-  // let repr = {key_size_repr = curr_g_key_size; signing_pub_key_repr = curr_g_key; transcript = new_g_transcript};
-
-  // //Do the state change
-  // let new_state = (Recv_no_sign_resp new_st);
-  
-  // assume_ (pure (g_transcript_non_empty repr.transcript));
-  // assume_ (pure (valid_transition tr0 (G_Recv_no_sign_resp repr)));
-  // let tr1 = next_trace tr0 (G_Recv_no_sign_resp repr);
-  
-  // assert (pure (G_Recv_no_sign_resp? (current_state tr1)));
-  // assert (pure (valid_transition tr0 (current_state tr1)));
-  // assert (pure (tr1 == next_trace tr0 (current_state tr1)));
-  // assert (pure(g_transcript_current_session_grows_by (current_transcript tr0 ) 
-  //                                               (current_transcript tr1) 
-  //                                               (Seq.append b_req b_resp)));
-  // //Call parser to parse and get the measurement blocks.
-
-  // let parser_res = parser req_param1 req_param2 resp_size m_spec req_context resp;
-
-  // let parser_res_result = parser_res.status;
-  // let parser_res_measurement_block_count = parser_res.measurement_block_count;
-  // let parser_res_measurement_block_vector = parser_res.measurement_block_vector;
-  // match parser_res_result {
-  //   Parse_error -> {
-      
-  //     admit() //(parser_res,new_state)
-  //   }
-  //   Signature_verification_error -> {
-     
-  //     admit()//unreachable ()
-  //   }
-  //   Success -> {
-  //     admit()
-  //   }
-  
-  // }
-}
-
-fn no_sign_resp3
-  (req_param1: u8)
-  (req_param2 : u8)
-  (m_spec: u8) 
-  (req_context: Seq.seq u8{Seq.length req_context == 8})
-  (req_size: u32)
-  (resp_size: u32)
-  (req:V.vec u8 { V.length req == u32_v req_size })
-  (resp:V.vec u8 { V.length resp == u32_v resp_size })
   (c:state)
   (#tr0:trace{has_full_state_info (current_state tr0)})
   (#b_resp: Seq.seq u8)
@@ -356,41 +220,65 @@ fn no_sign_resp3
   (#p_req : perm)
   (#p_resp:perm)
    requires (V.pts_to req #p_req b_req **
-             V.pts_to resp #p_resp b_resp) **
-             spdm_inv c trace_ref tr0 **
+             V.pts_to ctx.resp #p_resp b_resp) **
+             spdm_inv c ((get_state_data c).g_trace_ref) tr0 **
              pure (G_Recv_no_sign_resp? (current_state tr0) \/ G_Initialized? (current_state tr0))
     returns res: spdm_measurement_result_t & state
     
     ensures V.pts_to req #p_req b_req **
-            V.pts_to resp #p_resp b_resp **
-            (let measurement_block_count = (fst res).measurement_block_count in
-            let result = (fst res).status in
-                  (match result with
-                    | Parse_error -> pure True
-                    | Signature_verification_error -> pure False
-                    | Success ->
-                              //parser post-condition 
-                              (exists* resp_repr. valid_resp_bytes req_param1 req_param2 m_spec req_context b_resp resp_repr **
-                                       valid_measurement_blocks req_param2 m_spec (fst res).measurement_block_vector resp_repr.measurement_record) **
-                              
-                              //state change related post-condition 
-                              (exists* r tr1. valid_resp req_param1 req_param2 m_spec req_context resp r **
-                                        spdm_inv c trace_ref tr1 **
-                                         (pure ((G_Recv_no_sign_resp? (current_state tr1) /\
-                                                 valid_transition tr0 (current_state tr1) /\ tr1 == next_trace tr0 (current_state tr1)) /\
-                                                 (G_Recv_no_sign_resp? (current_state tr1) /\
-                                               
-                                                  g_transcript_current_session_grows_by (current_transcript tr0 ) 
-                                                                                     (current_transcript tr1) 
-                                                                                     (Seq.append b_req b_resp))))
-)))
+            V.pts_to ctx.resp #p_resp b_resp **
+
+            //parser related post-conditions
+            parser_post ctx (fst res) #b_resp **
+            //state change related post-condition 
+            (exists* r tr1. no_sign_resp_state_related_post_conditions ctx r tr0 tr1 c (snd res) #b_resp #b_req)
 {
+  //current state transcript
+  (*let curr_state_data = get_state_data c;
+  let curr_state_transcript = get_state_data_transcript curr_state_data;
+  let curr_state_signing_pub_key = get_state_data_signing_pub_key curr_state_data;
+  let curr_state_key_size = get_state_data_key_size curr_state_data;
+
   
-  assert_ (V.pts_to resp #p_resp b_resp);
+  //append req and resp
+  let append_req_resp = append_vec req resp #b_req #b_resp #p_req #p_resp;
+  
+  //get the ghost transcript
+  let curr_g_transcript = current_transcript tr0;
+  let curr_g_key = current_key tr0;
+  let curr_g_key_size = current_key_size tr0;
+  //unfold (spdm_inv c trace_ref tr0);
+  
+  //unfold (session_state_related c (current_state tr0));
+
+  assume_(V.pts_to curr_state_transcript (G.reveal curr_g_transcript));
+  //append req/resp to the current trascript
+  let new_transcript = append_vec curr_state_transcript append_req_resp #curr_g_transcript #(Seq.append b_req b_resp);
+  let new_g_transcript = g_append curr_g_transcript (Seq.append b_req b_resp);
+  //create a new state data record with the new transcript
+  assume_ (pure (V.length curr_state_signing_pub_key == u32_v curr_state_key_size));
+
+  let new_st = {key_size = curr_state_key_size; signing_pub_key = curr_state_signing_pub_key; session_transcript = new_transcript };
+  
+  ////creation of the ghost session data storage
+  let repr = {key_size_repr = curr_g_key_size; signing_pub_key_repr = curr_g_key; transcript = new_g_transcript};
+
+  //Do the state change
+  let new_state = (Recv_no_sign_resp new_st);
+  
+  assume_ (pure (g_transcript_non_empty repr.transcript));
+  assume_ (pure (valid_transition tr0 (G_Recv_no_sign_resp repr)));
+  let tr1 = next_trace tr0 (G_Recv_no_sign_resp repr);
+  
+  assert (pure (G_Recv_no_sign_resp? (current_state tr1)));
+  assert (pure (valid_transition tr0 (current_state tr1)));
+  assert (pure (tr1 == next_trace tr0 (current_state tr1)));
+  assert (pure(g_transcript_current_session_grows_by (current_transcript tr0 ) 
+                                                (current_transcript tr1) 
+                                                (Seq.append b_req b_resp)));
+  //Call parser to parse and get the measurement blocks.
 
   let parser_res = parser req_param1 req_param2 resp_size m_spec req_context resp;
-
-  assert_ (V.pts_to resp #p_resp b_resp);
 
   let parser_res_result = parser_res.status;
   let parser_res_measurement_block_count = parser_res.measurement_block_count;
@@ -402,73 +290,13 @@ fn no_sign_resp3
     }
     Signature_verification_error -> {
      
-      admit()
+      admit()//unreachable ()
     }
     Success -> {
-      //current state transcript
-      let curr_state_data = get_state_data c;
-      let curr_state_transcript = get_state_data_transcript curr_state_data;
-      let curr_state_signing_pub_key = get_state_data_signing_pub_key curr_state_data;
-      let curr_state_key_size = get_state_data_key_size curr_state_data;
-
-
-      
-      (*current context here, 
-       Current context:
-         V.pts_to req b_req **
-         V.pts_to resp (G.reveal b_resp) **
-         spdm_inv c trace_ref tr0 ***)
-      
-      (*In the original pre-condition, 
-          V.pts_to resp #p_resp b_resp*)
-      
-      (*in the parser post-condition,
-         V.pts_to resp #p_resp b_resp*)
-
-      (*The assert is failing as well as why the parser post condition is not holding?*)
-      //assert_ (V.pts_to resp #p_resp b_resp);
-      
-      //append req and resp
-      (*let append_req_resp = append_vec req resp #b_req #b_resp #p_req #p_resp;
-  
-      //get the ghost transcript
-      let curr_g_transcript = current_transcript tr0;
-      let curr_g_key = current_key tr0;
-      let curr_g_key_size = current_key_size tr0;
-      //unfold (spdm_inv c trace_ref tr0);
-  
-      //unfold (session_state_related c (current_state tr0));
-
-      assume_(V.pts_to curr_state_transcript (G.reveal curr_g_transcript));
-      //append req/resp to the current trascript
-      let new_transcript = append_vec curr_state_transcript append_req_resp #curr_g_transcript #(Seq.append b_req b_resp);
-      let new_g_transcript = g_append curr_g_transcript (Seq.append b_req b_resp);
-      //create a new state data record with the new transcript
-      assume_ (pure (V.length curr_state_signing_pub_key == u32_v curr_state_key_size));
-
-      let new_st = {key_size = curr_state_key_size; signing_pub_key = curr_state_signing_pub_key; session_transcript = new_transcript };
-  
-      ////creation of the ghost session data storage
-      let repr = {key_size_repr = curr_g_key_size; signing_pub_key_repr = curr_g_key; transcript = new_g_transcript};
-
-      //Do the state change
-      let new_state = (Recv_no_sign_resp new_st);
-  
-      assume_ (pure (g_transcript_non_empty repr.transcript));
-      assume_ (pure (valid_transition tr0 (G_Recv_no_sign_resp repr)));
-      let tr1 = next_trace tr0 (G_Recv_no_sign_resp repr);
-  
-      assert (pure (G_Recv_no_sign_resp? (current_state tr1)));
-      assert (pure (valid_transition tr0 (current_state tr1)));
-      assert (pure (tr1 == next_trace tr0 (current_state tr1)));
-      assert (pure(g_transcript_current_session_grows_by (current_transcript tr0 ) 
-                                                (current_transcript tr1) 
-                                                (Seq.append b_req b_resp)));*)
-  
       admit()
     }
   
-  }
+  }*)
+  admit()
 }
-
 
